Zcash/Circuits/Integration.lean
@@ -1,6 +1,5 @@
 import Zcash.Circuits.Integration.ActionCopyWitness
 import Zcash.Circuits.Integration.ActionEncoding
-import Zcash.Circuits.Integration.ActionFixedCoherence
 import Zcash.Circuits.Integration.ActionConstraintBounds
 import Zcash.Circuits.Integration.ActionCorrectness
 import Zcash.Circuits.Integration.ActionPermutationDomain
